word to list to word

opentheory/examples/word.ml
@@ -18,7 +18,30 @@ let word_size_nonzero = prove
 
 export_thm word_size_nonzero;;
 
-(* Apply theory functor modular *)
+(* Start of parametric theory instantiation: modular *)
+
+(* modular-mod *)
+
+let lt_word_size = new_axiom
+  `!n. n < word_size ==> n MOD word_size = n`;;
+
+let word_size_lt = new_axiom
+  `!n. n MOD word_size < word_size`;;
+
+let mod_mod_word_size = new_axiom
+  `!n. n MOD word_size MOD word_size = n MOD word_size`;;
+
+let add_mod_word_size = new_axiom
+  `!m n.
+     (m MOD word_size + n MOD word_size) MOD word_size =
+     (m + n) MOD word_size`;;
+
+let mult_mod_word_size = new_axiom
+  `!m n.
+     (m MOD word_size * n MOD word_size) MOD word_size =
+     (m * n) MOD word_size`;;
+
+(* modular-def *)
 
 new_type ("word",0);;
 
@@ -35,16 +58,20 @@ let word_to_num_to_word = new_axiom
   `!x. num_to_word (word_to_num x) = x`;;
 
 let num_to_word_inj = new_axiom
-  `!x y. x < word_size /\ y < word_size /\ num_to_word x = num_to_word y ==> x = y`;;
+  `!x y.
+     x < word_size /\ y < word_size /\ num_to_word x = num_to_word y ==>
+     x = y`;;
 
 let num_to_word_to_num = new_axiom
   `!x. word_to_num (num_to_word x) = x MOD word_size`;;
 
 let num_to_word_add = new_axiom
-  `!x1 y1. num_to_word (x1 + y1) = word_add (num_to_word x1) (num_to_word y1)`;;
+  `!x1 y1.
+     num_to_word (x1 + y1) = word_add (num_to_word x1) (num_to_word y1)`;;
 
 let num_to_word_mult = new_axiom
-  `!x1 y1. num_to_word (x1 * y1) = word_mult (num_to_word x1) (num_to_word y1)`;;
+  `!x1 y1.
+     num_to_word (x1 * y1) = word_mult (num_to_word x1) (num_to_word y1)`;;
 
 let word_neg_def = new_axiom
   `!x. word_neg x = num_to_word (word_size - word_to_num x)`;;
@@ -58,6 +85,8 @@ let word_le_def = new_axiom
 let word_lt_def = new_axiom
   `!x y. word_lt x y = ~(word_le y x)`;;
 
+(* modular-thm *)
+
 let word_to_num_inj = new_axiom
   `!x y. word_to_num x = word_to_num y ==> x = y`;;
 
@@ -67,10 +96,20 @@ let num_to_word_eq = new_axiom
 let word_to_num_bound = new_axiom
   `!x. word_to_num x < word_size`;;
 
+let word_to_num_div_bound = new_axiom
+  `!x. word_to_num x DIV word_size = 0`;;
+
+let word_add_to_num = new_axiom
+  `!x y.
+     word_to_num (word_add x y) =
+     (word_to_num x + word_to_num y) MOD word_size`;;
+
+(* End of parametric theory instantiation: modular *)
+
 logfile "word-bits-def";;
 
 let word_shl_def = new_definition
- `!w n. word_shl w n = num_to_word (word_to_num w * (2 EXP n))`;;
+ `!w n. word_shl w n = num_to_word ((2 EXP n) * word_to_num w)`;;
 
 export_thm word_shl_def;;
 
@@ -98,6 +137,11 @@ let list_to_word_def = new_recursive_definition list_RECURSION
 
 export_thm list_to_word_def;;
 
+let is_word_list_def = new_definition
+ `!l. is_word_list (l : bool list) <=> LENGTH l = word_width`;;
+
+export_thm is_word_list_def;;
+
 let word_and_def = new_definition
   `!w1 w2.
      word_and w1 w2 =
@@ -119,11 +163,138 @@ export_thm word_not_def;;
 
 logfile "word-bits-thm";;
 
-let length_word_to_list = prove
-  (`!w. LENGTH (word_to_list w) = word_width`,
-   REWRITE_TAC [word_to_list_def; LENGTH_MAP; length_interval]);;
+let is_word_to_list = prove
+  (`!w. is_word_list (word_to_list w)`,
+   REWRITE_TAC
+     [is_word_list_def; word_to_list_def; LENGTH_MAP; length_interval]);;
 
-export_thm length_word_to_list;;
+export_thm is_word_to_list;;
+
+let PAT_ASSUM pat =
+    let is_pat th = can (term_match [] pat) (concl th) in
+    FIRST_X_ASSUM (fun th -> if is_pat th then MP_TAC th else NO_TAC);;
+
+let KNOW_TAC =
+    let th = ITAUT `!x y. x /\ (x ==> y) ==> y` in
+    fun tm ->
+      MATCH_MP_TAC th THEN
+      EXISTS_TAC tm THEN
+      CONJ_TAC;;
+
+let cond_mod_2 = prove
+  (`!n. (if ODD n then 1 else 0) = n MOD 2`,
+   GEN_TAC THEN
+   MP_TAC (SPEC `n:num` EVEN_OR_ODD) THEN
+   STRIP_TAC THENL
+   [MP_TAC (SPEC `n:num` EVEN_MOD) THEN
+    ASM_REWRITE_TAC [] THEN
+    DISCH_THEN (fun th -> REWRITE_TAC [th]) THEN
+    MP_TAC (SPEC `n:num` NOT_ODD) THEN
+    ASM_REWRITE_TAC [] THEN
+    DISCH_THEN (fun th -> REWRITE_TAC [th]);
+    MP_TAC (SPEC `n:num` ODD_MOD) THEN
+    ASM_REWRITE_TAC [] THEN
+    DISCH_THEN (fun th -> REWRITE_TAC [th])]);;
+
+let word_bit_mod_2 = prove
+  (`!w n.
+      (if word_bit w n then 1 else 0) =
+      (word_to_num w DIV (2 EXP n)) MOD 2`,
+   REWRITE_TAC [word_bit_def; word_shr_def; num_to_word_to_num; cond_mod_2] THEN
+   REPEAT GEN_TAC THEN
+   AP_THM_TAC THEN
+   AP_TERM_TAC THEN
+   MATCH_MP_TAC lt_word_size THEN
+   MATCH_MP_TAC LET_TRANS THEN
+   EXISTS_TAC `word_to_num w` THEN
+   CONJ_TAC THENL
+   [MATCH_MP_TAC DIV_LE THEN
+    REWRITE_TAC [EXP_EQ_0] THEN
+    NUM_REDUCE_TAC;
+    REWRITE_TAC [word_to_num_bound]]);;
+
+let nil_to_word_to_num = prove
+  (`word_to_num (list_to_word []) = 0`,
+   REWRITE_TAC [list_to_word_def; num_to_word_to_num] THEN
+   MATCH_MP_TAC lt_word_size THEN
+   REWRITE_TAC [LT_NZ; word_size_nonzero]);;
+
+export_thm nil_to_word_to_num;;
+
+let cons_to_word_to_num = prove
+  (`!h t.
+      word_to_num (list_to_word (CONS h t)) =
+      (2 * word_to_num (list_to_word t) + (if h then 1 else 0)) MOD word_size`,
+   REWRITE_TAC [list_to_word_def] THEN
+   REPEAT STRIP_TAC THEN
+   MP_TAC (SPEC `h : bool` BOOL_CASES_AX) THEN
+   STRIP_TAC THENL
+   [ASM_REWRITE_TAC
+      [word_add_to_num; word_shl_def; EXP_1; word_to_num_to_word] THEN
+    REWRITE_TAC [num_to_word_to_num; add_mod_word_size];
+    ASM_REWRITE_TAC [word_shl_def; EXP_1; word_to_num_to_word; ADD_0] THEN
+    REWRITE_TAC [num_to_word_to_num; add_mod_word_size]]);;
+
+export_thm cons_to_word_to_num;;
+
+let word_to_list_to_word = prove
+  (`!w. list_to_word (word_to_list w) = w`,
+   GEN_TAC THEN
+   REWRITE_TAC [word_to_list_def] THEN
+   MATCH_MP_TAC word_to_num_inj THEN
+   MATCH_MP_TAC (ITAUT`!p q. (p ==> q) /\ p ==> q`) THEN
+   EXISTS_TAC
+     `!k.
+        k <= word_width ==>
+        word_to_num
+          (list_to_word (MAP (word_bit w) (interval (word_width - k) k))) =
+          word_to_num w DIV (2 EXP (word_width - k))` THEN
+   CONJ_TAC THENL
+   [DISCH_THEN (MP_TAC o SPEC `word_width`) THEN
+    REWRITE_TAC [SUB_REFL; LE_REFL; EXP; DIV_1];
+    MATCH_MP_TAC num_INDUCTION THEN
+    CONJ_TAC THENL
+    [REWRITE_TAC
+       [SUB; interval_def; MAP; nil_to_word_to_num; GSYM word_size_def;
+        word_to_num_div_bound];
+     REPEAT STRIP_TAC THEN
+     PAT_ASSUM `X ==> Y` THEN
+     MATCH_MP_TAC (ITAUT `X /\ (Y ==> Z) ==> ((X ==> Y) ==> Z)`) THEN
+     CONJ_TAC THENL
+     [MATCH_MP_TAC LE_TRANS THEN
+      EXISTS_TAC `SUC k` THEN
+      ASM_REWRITE_TAC [LE; LE_REFL];
+      REWRITE_TAC [interval_def; MAP; cons_to_word_to_num] THEN
+      KNOW_TAC `word_width - k = SUC (word_width - SUC k)` THENL
+      [ASM_ARITH_TAC;
+       DISCH_THEN (fun th -> REWRITE_TAC [th]) THEN
+       DISCH_THEN (fun th -> REWRITE_TAC [th]) THEN
+       REWRITE_TAC [word_bit_mod_2] THEN
+       ONCE_REWRITE_TAC [MULT_SYM] THEN
+       REWRITE_TAC [EXP] THEN
+       MP_TAC (SPECL [`word_to_num w`; `2 EXP (word_width - SUC k)`;
+                       `2`] (ONCE_REWRITE_RULE [MULT_SYM] DIV_DIV)) THEN
+       MATCH_MP_TAC (ITAUT `X /\ (Y ==> Z) ==> ((X ==> Y) ==> Z)`) THEN
+       CONJ_TAC THENL
+       [REWRITE_TAC [GSYM EXP; EXP_EQ_0] THEN
+        NUM_REDUCE_TAC;
+        DISCH_THEN (fun th -> REWRITE_TAC [GSYM th]) THEN
+        MP_TAC (SPECL [`word_to_num w DIV (2 EXP (word_width - SUC k))`;
+                        `2`] DIVISION) THEN
+        MATCH_MP_TAC (ITAUT `X /\ (Y ==> Z) ==> ((X ==> Y) ==> Z)`) THEN
+        CONJ_TAC THENL
+        [NUM_REDUCE_TAC;
+         DISCH_THEN (fun th -> REWRITE_TAC [GSYM (CONJUNCT1 th)]) THEN
+         MATCH_MP_TAC lt_word_size THEN
+         MATCH_MP_TAC LET_TRANS THEN
+         EXISTS_TAC `word_to_num w` THEN
+         CONJ_TAC THENL
+         [MATCH_MP_TAC DIV_LE THEN
+          REWRITE_TAC [EXP_EQ_0] THEN
+          NUM_REDUCE_TAC;
+          REWRITE_TAC [word_to_num_bound]]]]]]]]);;
+
+export_thm word_to_list_to_word;;
 
 (***
 let list_to_word_to_list = prove
